Convert exp from using set to finset
This is in preparation for getting fresh variables from a finset.

exp.lean
@@ -1,8 +1,9 @@
-import data.set
+import data.finset
 
-open set
+open finset
+open nat
 
-inductive exp : set ℕ → Type :=
-  | var : Π {X}  x, x ∈ X            → exp X
-  | app : Π {X}   , exp X → exp X    → exp X
-  | lam : Π {X}  x, exp (insert x X) → exp X
+inductive exp : finset ℕ → Type :=
+  | var : Π {X} x, x ∈ X            → exp X
+  | app : Π {X}  , exp X → exp X    → exp X
+  | lam : Π {X} x, exp (insert x X) → exp X
